Add ability to track/check pc and bytecode.

src/dafny/evms/mini-evm-with-gas.dfy
@@ -12,12 +12,13 @@
  * under the License.
  */
 
-
 include "../utils/NativeTypes.dfy"
 include "../utils/NonNativeTypes.dfy"
+include "./EVMOpcodes.dfy"
 
 import opened NativeTypes
 import opened NonNativeTypes
+import opened EVMOpcodes
 
 /** The type for the EVM stack. 
  * 
@@ -38,61 +39,88 @@ class EVM {
     /** The gas left in the EVM.  */
     var gas: uint256
 
+    /** The program counter. */
+    var pc: nat 
+
     /** Enable/disable gas check. */
     const checkGas: bool
+
+    /** Enable/disable bytecode checking. */
+    const checkCode: bool
+
+    /** The optional (can be empty sequence) bytecode. */
+    const code: seq<uint8>
 
     /** Init the VM. 
      *  
      *  @param  g       Initial gas in the EVM.add
      *  @param  check   Whether the machine requires gas or not.
+     *  @param  c       The bytecode.
+     *
+     *  @note           If bytecode not empty, every execution of an instruction
+     *                  is checked against the bytecode.
+     *  @example        c = [PUSH1, 2]
+     *                  this.push(v) can only be executed if current pc is such that code[pc] is PUSH1
+     *                  and code[pc + 1] == v 
      */
-    constructor (g: uint256, check: bool) 
+    constructor (g: uint256, check: bool, c: seq<uint8> := []) 
         ensures stack == []
         ensures gas == g 
         ensures checkGas == check
+        ensures pc == 0
+        ensures checkCode == (|c| > 0)
+        ensures code == c
     {
+        pc := 0;
         stack := []; 
         gas := g;
         checkGas := check;
+        code := c;
+        checkCode := |c| > 0;
     }
 
+    //  The semantics of the following instructions are
+    //  defined by their pre- and post-conditions.
+
     /** 
-     *  PUSH opcode.
-     *  This is code for push32 but as other pushes 
-     *  are syntactic sugar we implement only this one.
+     *  PUSH1 opcode.
      *
      *  @param  v   The value to push on the stack.
-     *  @return     Add `v` to the top of the stack.
+     *  @return     Add `v` to the top of the stack (and convert to uint256).
      */
-    method push(v: uint256) 
+    method push(v: uint8) 
         requires !checkGas || gas >= 1
-
+        requires !checkCode || (pc + 1 < |code| && code[pc] == PUSH1 && code[pc + 1] == v) 
         ensures |stack| == |old(stack)| + 1
-        ensures stack == [v] + old(stack)
+        ensures stack == [v as uint256] + old(stack)
         ensures !checkGas || gas == old(gas) - 1
+        ensures pc == old(pc) + 2
 
-        modifies `stack, `gas
+        modifies this
     {
-        stack := [v] + stack;
+        stack := [v as uint256] + stack;
         gas := gas - (if checkGas then 1 else 0);
+        pc := pc + 2;
     }
 
     /**
      *  POP opcode.
-     *  @return     The tail of the stack.
      */
     method pop() 
         requires |stack| > 0 
         requires !checkGas || gas >= 1
+        requires !checkCode || (pc < |code| && code[pc] == POP) 
 
         ensures |stack| == |old(stack)| - 1
         ensures stack == old(stack[1..])
         ensures !checkGas || gas == old(gas) - 1
+        ensures pc == old(pc) + 1
 
-        modifies `stack, `gas
+        modifies this
     {
         stack := stack[1..];
         gas := gas - (if checkGas then 1 else 0);
+        pc := pc + 1;
     }
 
     /**
@@ -101,62 +129,65 @@ class EVM {
     method swap1()  
         requires |stack| >= 2
         requires !checkGas || gas >= 1
+        requires !checkCode || (pc < |code| && code[pc] == SWAP1) 
 
         ensures |stack| == |old(stack)|
         ensures stack[0] == old(stack[1])
         ensures stack[1] == old(stack[0])
         ensures stack[2..] == old(stack[2..])
         ensures !checkGas || gas == old(gas) - 1
+        ensures pc == old(pc) + 1
 
-        modifies `stack, `gas
+        modifies this
     {
         stack := [stack[1]] + [stack[0]] + stack[2..];
         gas := gas - (if checkGas then 1 else 0);
+        pc := pc + 1;
     }
 
 
     /**
      *  ADD opcode.
-     *  
-     *  Assume stack = [a,b] + xr
-     *  @returns [a + b] + xr
      */
     method add()  
         requires |stack| >= 2
         requires stack[0] as nat + stack[1] as nat <= MAX_UINT256
         requires !checkGas || gas >= 1
+        requires !checkCode || (pc < |code| && code[pc] == ADD) 
 
         ensures |stack| == |old(stack)| - 1
         ensures stack[0] == old(stack)[0] + old(stack)[1]
         ensures stack[1..] == old(stack[2..])
         ensures !checkGas || gas == old(gas) - 1
+        ensures pc == old(pc) + 1
 
-        modifies `stack, `gas
+        modifies this
     {
         stack := [stack[0] + stack[1]] + stack[2..];
         gas := gas - (if checkGas then 1 else 0);
+        pc := pc + 1;
     }
 
     /**
      *  SUB opcode. compute stack[1] - stack[0], which is not the semantics
      *  of SUB that is stack[0] - stack[1]
      */
-    method subR()  
-        requires |stack| >= 2
-        requires stack[1] as nat - stack[0] as nat >= 0
-        requires !checkGas || gas >= 1
+    // method subR()  
+    //     requires |stack| >= 2
+    //     requires stack[1] as nat - stack[0] as nat >= 0
+    //     requires !checkGas || gas >= 1
 
-        ensures |stack| == |old(stack)| - 1
-        ensures stack[0] == old(stack)[1] - old(stack)[0]
-        ensures stack[1..] == old(stack)[2..]
-        ensures !checkGas || gas == old(gas) - 1
+    //     ensures |stack| == |old(stack)| - 1
+    //     ensures stack[0] == old(stack)[1] - old(stack)[0]
+    //     ensures stack[1..] == old(stack)[2..]
+    //     ensures !checkGas || gas == old(gas) - 1
 
-        modifies `stack, `gas
-        // modifies if checkGas then {`stack, `gas} else {this`stack} 
-    {
-        stack := [stack[1] - stack[0]] + stack[2..];
-        gas := gas - (if checkGas then 1 else 0);
-    }
+    //     modifies `stack, `gas
+    //     // modifies if checkGas then {`stack, `gas} else {this`stack} 
+    // {
+    //     stack := [stack[1] - stack[0]] + stack[2..];
+    //     gas := gas - (if checkGas then 1 else 0);
+    // }
 
     /**
      *  SUB opcode. compute stack[0] - stack[1], which is the
@@ -169,17 +200,40 @@ class EVM {
         requires |stack| >= 2
         requires stack[0] as nat - stack[1] as nat >= 0
         requires !checkGas || gas >= 1
+        requires !checkCode || (pc < |code| && code[pc] == SUB) 
 
         ensures |stack| == |old(stack)| - 1
         ensures stack[0] == old(stack)[0] - old(stack)[1]
         ensures stack[1..] == old(stack)[2..]
         ensures !checkGas || gas == old(gas) - 1
+        ensures pc == old(pc) + 1
 
-        modifies `stack, `gas 
+        modifies this 
     {
         stack := [stack[0] - stack[1]] + stack[2..];
         gas := gas - (if checkGas then 1 else 0);
+        pc := pc + 1;
     }
+    /**
+     *  DUP1 opcode. Duplicate the second element of the stack.
+     */
+    method dup1()  
+        requires |stack| >= 1
+        requires !checkGas || gas >= 1
+        requires !checkCode || (pc < |code| && code[pc] == DUP1) 
+
+        ensures |stack| == |old(stack)| + 1
+        ensures stack == [old(stack)[0]] + old(stack)
+        ensures !checkGas || gas == old(gas) - 1
+        ensures pc == old(pc) + 1
+
+        modifies this
+    {
+        stack := [stack[0]] + stack;
+        gas := gas - (if checkGas then 1 else 0);
+        pc := pc + 1;
+    }
+
 
     /**
      *  DUP2 opcode. Duplicate the second element of the stack.
@@ -187,15 +241,18 @@ class EVM {
     method dup2()  
         requires |stack| >= 2
         requires !checkGas || gas >= 1
+        requires !checkCode || (pc < |code| && code[pc] == DUP2) 
 
         ensures |stack| == |old(stack)| + 1
         ensures stack == [old(stack)[1]] + old(stack)
         ensures !checkGas || gas == old(gas) - 1
+        ensures pc == old(pc) + 1
 
-        modifies `stack, `gas
+        modifies this
     {
         stack := [stack[1]] + stack;
         gas := gas - (if checkGas then 1 else 0);
+        pc := pc + 1;
     }
 
     /**
@@ -205,38 +262,116 @@ class EVM {
      *  Assume  stack
      *  @returns [stack[i]] + stack
      */
-    method dup(i: nat)
-        requires 0 <= i <= 15  
-        requires |stack| > i as nat
-        requires !checkGas || gas >= 1
+    // method dup(i: nat)
+    //     requires 0 <= i <= 15  
+    //     requires |stack| > i as nat
+    //     requires !checkGas || gas >= 1
+    //     requires !checkCode || (pc < |code| && code[pc] == 0x07) 
 
-        ensures |stack| == |old(stack)| + 1
-        ensures stack == [old(stack)[i]] + old(stack)
-        ensures !checkGas || gas == old(gas) - 1
+    //     ensures |stack| == |old(stack)| + 1
+    //     ensures stack == [old(stack)[i]] + old(stack)
+    //     ensures !checkGas || gas == old(gas) - 1
+    //     ensures pc == old(pc) + 1
 
-        modifies `stack, `gas
-    {
-        stack := [stack[i]] + stack;
-        gas := gas - (if checkGas then 1 else 0);
-    }
-
+    //     modifies this
+    // {
+    //     stack := [stack[i]] + stack;
+    //     gas := gas - (if checkGas then 1 else 0);
+    //     pc := pc + 1;
+    // }
 
     /**
      *  GT opcode. Compute stack[0] > stack[1] and store result. 
-     *
-     *  
      */
     method gt()  
         requires |stack| >= 2
         requires !checkGas || gas >= 1
+        requires !checkCode || (pc < |code| && code[pc] == GT) 
 
         ensures |stack| == |old(stack)| - 1
         ensures stack == [if (old(stack)[0] > old(stack)[1]) then 1 else 0] + old(stack)[2..]
         ensures !checkGas || gas == old(gas) - 1
+        ensures pc == old(pc) + 1 
 
-        modifies `stack, `gas
+        modifies this
     {
         stack := (if (stack[0] > stack[1]) then [1] else [0]) + stack[2..];
+        gas := gas - (if checkGas then 1 else 0);
+        pc := pc + 1;
+    }
+
+    /**
+     *  JUMPI opcode.
+     *  JUMPI uses the top of the stack to determine where to branch.
+     *  JUMPI destination condition
+     */
+    method jumpi()  
+        requires |stack| >= 2
+        requires !checkGas || gas >= 1
+        requires !checkCode || (pc < |code| && code[pc] == JUMPI) 
+
+        ensures |stack| == |old(stack)| - 2
+        ensures stack == old(stack)[2..]
+        ensures !checkGas || gas == old(gas) - 1
+        ensures pc == if old(stack[1]) != 0 then old(stack[0]) as nat else old(pc) + 1 
+
+        modifies this
+    {
+        pc := if stack[1] != 0 then stack[0] as nat else pc + 1 ;
+        stack := stack[2..];
+        gas := gas - (if checkGas then 1 else 0);
+    }
+
+    method jump()  
+        requires |stack| >= 1
+        requires !checkGas || gas >= 1
+        requires !checkCode || (pc < |code| && code[pc] == JUMP) 
+
+        ensures |stack| == |old(stack)| - 1
+        ensures stack == old(stack)[1..]
+        ensures !checkGas || gas == old(gas) - 1
+        ensures pc == old(stack[0]) as nat
+
+        modifies this
+    {
+        pc := stack[0] as nat ;
+        stack := stack[1..];
+        gas := gas - (if checkGas then 1 else 0);
+    }
+
+    method iszero()  
+        requires |stack| >= 1
+        requires !checkGas || gas >= 1
+        requires !checkCode || (pc < |code| && code[pc] == ISZERO) 
+
+        ensures |stack| == |old(stack)|
+        ensures stack == [if old(stack[0]) == 0 then 1 else 0] + old(stack[1..])
+        ensures !checkGas || gas == old(gas) - 1
+        ensures pc == old(pc) + 1 
+        ensures stack[0] > 0 <==> old(stack[0]) == 0
+
+        modifies this
+    {
+        pc := pc + 1 ;
+        stack := [if stack[0] == 0 then 1 else 0] + stack[1..];
+        gas := gas - (if checkGas then 1 else 0);
+    }
+
+    method stop()  
+        // requires |stack| >= 1
+        requires !checkGas || gas >= 1
+        requires !checkCode || (pc < |code| && code[pc] == STOP) 
+
+        ensures |stack| == |old(stack)|
+        // ensures stack == [if old(stack[0]) == 0 then 1 else 0] + old(stack[1..])
+        ensures !checkGas || gas == old(gas) - 1
+        ensures pc == old(pc) + 1 
+        // ensures stack[0] > 0 <==> old(stack[0]) == 0
+
+        modifies this
+    {
+        pc := pc + 1 ;
+        // stack := [if stack[0] == 0 then 1 else 0] + stack[1..];
         gas := gas - (if checkGas then 1 else 0);
     }
 
@@ -251,27 +386,27 @@ class EVM {
      *  Counter must be one of the last 16 items pushed on the stack.
      *  
      */
-    method incr(i: nat, v: uint256)
-        requires 0 <= i <= 15
-        requires !checkGas || gas >= 3
-        requires |stack| > i as nat
-        requires stack[i] as nat + v as nat <= MAX_UINT256 
+    // method incr(i: nat, v: uint256)
+    //     requires 0 <= i <= 15
+    //     requires !checkGas || gas >= 3
+    //     requires |stack| > i as nat
+    //     requires stack[i] as nat + v as nat <= MAX_UINT256 
+    //     requires !checkCode
+    //     ensures |stack| == |old(stack)| + 1
+    //     ensures stack == [old(stack[i]) + v] + old(stack)
+    //     ensures stack[1..] == old(stack)
+    //     ensures !checkGas || gas == old(gas) - 3
 
-        ensures |stack| == |old(stack)| + 1
-        ensures stack == [old(stack[i]) + v] + old(stack)
-        ensures stack[1..] == old(stack)
-        ensures !checkGas || gas == old(gas) - 3
-
-        modifies `stack, `gas
-    {
-        //  Stack is [x_0, x_1, ..., x _i] + xs
-        //  put element i on top of stack
-        dup(i);
-        //  Stack is [x_i, x_0, x_1, ..., x _i] + xs
-        push(v);
-        // Stack is [v, x_i, x_0, x_1, ..., x _i] + xs
-        add();
-        // Stack is [x_i + v, x_0, x_1, ..., x _i] + xs
-    }
+    //     modifies this
+    // {
+    //     //  Stack is [x_0, x_1, ..., x _i] + xs
+    //     //  put element i on top of stack
+    //     dup(i);
+    //     //  Stack is [x_i, x_0, x_1, ..., x _i] + xs
+    //     push(v);
+    //     // Stack is [v, x_i, x_0, x_1, ..., x _i] + xs
+    //     add();
+    //     // Stack is [x_i + v, x_0, x_1, ..., x _i] + xs
+    // }
 
 }
